{
 "cells": [
  {
   "cell_type": "markdown",
   "metadata": {},
   "source": [
    "## 19. Causal Inference"
   ]
  },
  {
   "cell_type": "markdown",
   "metadata": {},
   "source": [
    "In this chapter we discuss causation.  Roughly speaking \"$X$ causes $Y$\" means that changing the value of $X$ will change the distribution of $Y$.  When $X$ causes $Y$, $X$ and $Y$ will be associated but the reverse is not, in general, true.\n",
    "\n",
    "We will consider two frameworks for discussing causation.  The first uses notation of **counterfactual** random variables.  The second, used in the next chapter, uses **directed acyclic graphs**."
   ]
  },
  {
   "cell_type": "markdown",
   "metadata": {},
   "source": [
    "### 19.1 The Counterfactual Model"
   ]
  },
  {
   "cell_type": "markdown",
   "metadata": {},
   "source": [
    "Suppose that $X$ is a binary treatment variable where $X = 1$ means \"treated\" and $X = 0$ means \"not treated\".\n",
    "\n",
    "Let $Y$ be some outcome variable such as the presence or absence of disease.  To distinguish the statement \"$X$ is associated with $Y$\" from the statement \"$X$ causes $Y$\" we need to enrich our probabilistic vocabulary.  We will decompose the response $Y$ into a more fine-grained object.\n",
    "\n",
    "We introduce two new random variables $(C_0, C_1)$ called **potential outcomes** with the following interpretation: $C_0$ is the outcome if the subject is not treated ($X = 0$) and $C_1$ is the outcome if the subject is treated ($X = 1$).  Then,\n",
    "\n",
    "$$ Y = \\begin{cases}\n",
    "C_0 & \\text{if } X = 0 \\\\\n",
    "C_1 & \\text{if } X = 1\n",
    "\\end{cases}$$"
   ]
  },
  {
   "cell_type": "markdown",
   "metadata": {},
   "source": [
    "We can express the relationship between $Y$ and $(C_0, C_1)$ more succintly by\n",
    "\n",
    "$$ Y = C_X $$\n",
    "\n",
    "This equation is called the **consistency relationship**."
   ]
  },
  {
   "cell_type": "markdown",
   "metadata": {},
   "source": [
    "Here is a toy dataset to make the relationship clear:\n",
    "\n",
    "$$\n",
    "\\begin{array}{cccc}\n",
    "X & Y & C_0 & C_1 \\\\\n",
    "\\hline\n",
    "0 & 4 & 4 & * \\\\\n",
    "0 & 7 & 7 & * \\\\\n",
    "0 & 2 & 2 & * \\\\\n",
    "0 & 8 & 8 & * \\\\\n",
    "\\hline\n",
    "1 & 3 & * & 3 \\\\\n",
    "1 & 5 & * & 5 \\\\\n",
    "1 & 8 & * & 8 \\\\\n",
    "1 & 9 & * & 9\n",
    "\\end{array}\n",
    "$$\n",
    "\n",
    "The asterisks denote unobserved values.  When $X = 0$ we don't observe $C_1$ in which case we say that $C_1$ is a **counterfactual** since it is the outcome you would have had if, counter to the fact, you had been treated ($X = 1$).  Similarly, when $X = 1$ we don't observe $C_0$ and we say that $C_0$ is counterfactual."
   ]
  },
  {
   "cell_type": "markdown",
   "metadata": {},
   "source": [
    "Notice that there are four types of subjects:\n",
    "\n",
    "$$\n",
    "\\begin{array}{lcc}\n",
    "\\text{Type} & C_0 & C_1 \\\\\n",
    "\\hline\n",
    "\\text{Survivors}       & 1 & 1 \\\\\n",
    "\\text{Responders}      & 0 & 1 \\\\\n",
    "\\text{Anti-responders} & 1 & 0 \\\\\n",
    "\\text{Doomed}          & 0 & 0\n",
    "\\end{array}\n",
    "$$\n",
    "\n",
    "Think of all of the potential outcomes $(C_0, C_1)$ as hidden variables that contain all the relevant information about the subject."
   ]
  },
  {
   "cell_type": "markdown",
   "metadata": {},
   "source": [
    "Define the **average causal effect** or **average treatment effect** to be\n",
    "\n",
    "$$ \\theta = \\mathbb{E}(C_1) - \\mathbb{E}(C_0) $$\n",
    "\n",
    "The parameter $\\theta$ has the following interpretation:  $\\theta$ is the mean if everyone were treated ($X = 1$) minus the mean if everyone were not treated ($X = 0$).  There are other ways of measuring the causal effect.  For example, if $C_0$ and $C_1$ are binary, we define the **causal odds ratio**\n",
    "\n",
    "$$ \\frac{\\mathbb{P}(C_1 = 1)}{\\mathbb{P}(C_1 = 0)} \\div \\frac{\\mathbb{P}(C_0 = 1)}{\\mathbb{P}(C_0 = 0)}$$\n",
    "\n",
    "and the **causal relative risk**\n",
    "\n",
    "$$ \\frac{\\mathbb{P}(C_1 = 1)}{\\mathbb{P}(C_0 = 1)} $$\n",
    "\n",
    "The main ideas will be the same whatever causal effect we use.  For simplicity, we shall work with the average causal effect $\\theta$."
   ]
  },
  {
   "cell_type": "markdown",
   "metadata": {},
   "source": [
    "Define the **association** to be\n",
    "\n",
    "$$ \\alpha = \\mathbb{E}(Y | X = 1) - \\mathbb{E}(Y | X = 0)$$\n",
    "\n",
    "Again we could use the odds ratio or other summaries if we wish."
   ]
  },
  {
   "cell_type": "markdown",
   "metadata": {},
   "source": [
    "**Theorem 19.1 (Association is not equal to Causation)**.  In general, $\\theta \\neq \\alpha$."
   ]
  },
  {
   "cell_type": "markdown",
   "metadata": {},
   "source": [
    "**Theorem 19.3**.  Suppose we randomly assign subjects to treatment and that $\\mathbb{P}(X = 0) > 0$ and $\\mathbb{P}(X = 1) > 0$.  Then $\\alpha = \\theta$.  Hence, any consistent estimator of $\\alpha$ is a consistent estimator of $\\theta$.  In particular, a consistent estimator is\n",
    "\n",
    "$$ \\hat{\\theta} = \\hat{\\mathbb{E}}(Y | X = 1) - \\hat{\\mathbb{E}}(Y | X = 0) = \\overline{Y}_1 - \\overline{Y}_0 $$\n",
    "\n",
    "is a consistent estimator of $\\theta$, where\n",
    "\n",
    "$$\n",
    "\\begin{array}{ll}\n",
    "\\hat{Y}_1 = \\frac{1}{n_1} \\sum_{i: X_i = 1} Y_i\n",
    "&\n",
    "\\hat{Y}_0 = \\frac{1}{n_0} \\sum_{i: X_i = 0} Y_i \\\\\n",
    "n_1 = \\sum_{i=1}^n X_i\n",
    "&\n",
    "n_0 = \\sum_{i=1}^n (1 - X_i)\n",
    "\\end{array}\n",
    "$$"
   ]
  },
  {
   "cell_type": "markdown",
   "metadata": {},
   "source": [
    "**Proof**.  Since $X$ is randomly assigned, $X$ is independent of $(C_0, C_1)$.  Hence,\n",
    "\n",
    "$$\n",
    "\\begin{align}\n",
    "\\theta &= \\mathbb{E}(C_1) - \\mathbb{E}(C_0) \\\\\n",
    "&= \\mathbb{E}(C_1 | X = 1) - \\mathbb{E}(C_0 | X = 0) \\\\\n",
    "&= \\mathbb{E}(Y | X = 1) - \\mathbb{E}(Y | X = 0) \\\\\n",
    "&= \\alpha\n",
    "\\end{align}\n",
    "$$\n",
    "\n",
    "The consistency follows from the law of large numbers."
   ]
  },
  {
   "cell_type": "markdown",
   "metadata": {},
   "source": [
    "If $Z$ is a covariate, we define the **conditional causal effect** by\n",
    "\n",
    "$$ \\theta_z = \\mathbb{E}(C_1 | Z = z) - \\mathbb{E}(C_0 | Z = z) $$\n",
    "\n",
    "In a randomized experiment, $\\theta_z = \\mathbb{E}(Y | X = 1, Z = z) - \\mathbb{E}(Y | X = 0, Z = z)$ and we can estimate the conditional causal effect using appropriate sample averages."
   ]
  },
  {
   "cell_type": "markdown",
   "metadata": {},
   "source": [
    "**Summary**\n",
    "\n",
    "- Random variables: $(C_0, C_1, X, Y)$\n",
    "- Consistency relationship: $Y = C_X$\n",
    "- Causal Effect: $\\theta = \\mathbb{E}(C_1) - \\mathbb{E}(C_0)$\n",
    "- Association: $\\alpha = \\mathbb{E}(Y | X = 1) - \\mathbb{E}(Y | X = 0)$\n",
    "- Random Assignment:  $(C_0, C_1) \\text{ тлл } X \\Longrightarrow \\theta = \\alpha$"
   ]
  },
  {
   "cell_type": "code",
   "execution_count": null,
   "metadata": {},
   "outputs": [],
   "source": []
  }
 ],
 "metadata": {
  "kernelspec": {
   "display_name": "Python 3",
   "language": "python",
   "name": "python3"
  },
  "language_info": {
   "codemirror_mode": {
    "name": "ipython",
    "version": 3
   },
   "file_extension": ".py",
   "mimetype": "text/x-python",
   "name": "python",
   "nbconvert_exporter": "python",
   "pygments_lexer": "ipython3",
   "version": "3.7.3"
  }
 },
 "nbformat": 4,
 "nbformat_minor": 2
}
